\begin{align*}
    D_0    & = \type~\Foo[\F~\Foo[\F]]~\interface~\br{~m(f~\F)~\F~}         \\
    D_1    & = \type~\BarType[\B~\BarType[\B]]~\interface~\br{~m(b~\B)~\B~} \\
    D_2    & = \type~\E[\F~\Foo[\F],~\B~\BarType[\B]]~\struct~\br{ }        \\
    D_3    & = \type~\T~\struct~\br{ }                                      \\
    D_4    & = \func~(t~\T)~m(t2~\T)~\T~\br{~\return~t~}                    \\
    \ov{D} & = \{D_0, D_1, D_2, D_3, D_4\}                                  \\
    e      & = \E[\T,~\T]\br{}
\end{align*}

The derivations for $D_0$, $D_1$, and $D_3$ were shown in previous examples.

\begin{mathpar}
    \derivrule[T-Specification]{
        \axiomrule{
            \distinct(t2)
        }
        \\
        \derivrule[T-Named]{
            (\type~\T~\struct~\br{ }) \in \ov{D}
        }{
            \emptyset \vdash \T \ok
        }
    }{
        \emptyset \vdash m(t2~\T)~\T \ok
    }

    \derivrule[T-Var]{
        \axiomrule{
            (t:\T) \in (t:\T,t2:\T)
        }
    }{
        \emptyset;t:\T,t2:\T \vdash t: \T
    }

    \derivrule[T-Func]{
        \axiomrule{
            \distinct(t,t2)
        }
        \\
        \axiomrule{
            \emptyset = \typeparams(\T)
        }
        \\
        \emptyset \vdash m(t2~\T)~\T \ok
        \\
        \emptyset;t:\T,t2:\T \vdash t: \T
        \\
        \axiomrule[$\imp_V$]{
            \T \imp \T
        }
    }{
        D_4 \ok
    }
\end{mathpar}

$(\F~\Foo[\F],~\B~\BarType[\B]) \vdash \Foo[\F] \ok$ can be derived analogously
to $(\F~\Foo[\F]) \vdash \Foo[\F] \ok$ in the previous example. The same applies
for $(\F~\Foo[\F],~\B~\BarType[\B]) \vdash \BarType[\B] \ok$.

\begin{mathpar}
    \derivrule[T-Formal]{
        \axiomrule{
            \distinct(\F,\B)
        }
        \\
        (\F~\Foo[\F],~\B~\BarType[\B]) \vdash \Foo[\F] \ok
        \\
        (\F~\Foo[\F],~\B~\BarType[\B]) \vdash \BarType[\B] \ok
    }{
        (\F~\Foo[\F],~\B~\BarType[\B]) \ok
    }

    \derivrule[T-Type]{
        (\F~\Foo[\F],~\B~\BarType[\B]) \ok
        \\
        \axiomrule{
            \F~\Foo[\F],~\B~\BarType[\B] \vdash \struct\br{} \ok
        }
        \\
        \axiomrule{
            \notcont(\E,~\struct\br{})
        }
    }{
        D_2 \ok
    }

    \derivrule{
        \axiomrule{
            \emptyset = \typeparams(\T)
        }
    }{
        \methods_\emptyset(T) = \br{~m(t2~\T)~\T~}
    }

    \derivrule{
        \derivrule{
            (\type~\Foo[\F~\Foo[\F]]~\interface~\br{~m(f~\F)~\F~}) \in \ov{D}
            \\
            \derivrule{
                \eta_5 = (\F \by \T)
            }{
                \eta_5 = (\F~\Foo[\F] \by \T)
            }
        }{
            \methods_\emptyset(\Foo[\T]) = \br{~m(f~\F)~\F~} \llbracket \eta_5 \rrbracket
        }
    }{
        \methods_\emptyset(\Foo[\T]) = \br{~m(f~\T)~\T~}
    }

\end{mathpar}

$\emptyset \vdash (\T \imp \BarType[\T])$ can be derived analogously to $\emptyset \vdash (\T \imp \Foo[\T])$.

\begin{mathpar}

    \derivrule{
        \derivrule[$\imp_I$]{
            \derivrule{
                \axiomrule{
                    \br{~m(t2~\T)~\T~} \supseteq \br{~m(f~\T)~\T~}
                }
            }{
                \methods_\emptyset(T) \supseteq \methods_\emptyset(\Foo[\T])
            }
        }{
            \emptyset \vdash (\T \imp \Foo[\T])
        }
    }{
        \emptyset \vdash (\F \imp \Foo[\F])[\eta_4]
    }

    \derivrule{
        \emptyset \vdash (\T \imp \BarType[\T])
    }{
        \emptyset \vdash (\B \imp \BarType[\B])[\eta_4]
    }

    \derivrule{
        \derivrule{
            \eta_4 = (\F \by \T,~\B \by \T)
        }{
            \eta_4 = (\F~\Foo[\F] \by \T,~\B~\BarType[\B] \by \T)
        }
        \\
        \emptyset \vdash (\F \imp \Foo[\F])[\eta_4]
        ~~~~
        \emptyset \vdash (\B \imp \BarType[\B])[\eta_4]
    }{
        \eta_4 = (\F~\Foo[\F] \by_\emptyset \T,~\B~\BarType[\B] \by_\emptyset \T)
    }

    \derivrule[T-Named]{
        \emptyset \vdash \T \ok
        \\
        \axiomrule{
            (\type~\E[\F~\Foo[\F],~\B~\BarType[\B]]~\struct~\br{ }) \in \ov{D}
        }
        \\
        \eta_4 = (\F~\Foo[\F] \by_\emptyset \T,~\B~\BarType[\B] \by_\emptyset \T)
    }{
        \emptyset \vdash \E[\T,\T] \ok
    }

    \derivrule[T-Struct-Literal]{
        \emptyset \vdash \E[\T,\T] \ok
    }{
        \emptyset;\emptyset \vdash \E[\T,\T]\br{} : \E[\T,\T]
    }
\end{mathpar}
